src/refinement/PromisingPF_AlgorithmicPF.v
@@ -22,9 +22,55 @@ Require Import Algorithmic.
 Set Implicit Arguments.
 
 
+Lemma no_promise_step
+      tid aeu1 aeu2
+      (STEP: AExecUnit.step tid aeu1 aeu2)
+      (WF: ExecUnit.wf tid aeu1)
+      (NOPROMISE: aeu1.(ExecUnit.local).(Local.promises) = bot):
+  <<NOPROMISE: aeu2.(ExecUnit.local).(Local.promises) = bot>> /\
+  <<TAINT: aeu2.(AExecUnit.aux).(AExecUnit.taint) = aeu1.(AExecUnit.aux).(AExecUnit.taint)>>.
+Proof.
+  destruct aeu1 as [[st1 lc1 mem1] aux1].
+  destruct aeu2 as [[st2 lc2 mem2] aux2].
+  ss. inv STEP.
+  - (* state_step *)
+    inv STEP0. ss. subst. inv LOCAL.
+    + inv LC. eauto.
+    + inv STEP. ss. destruct ex; ss.
+    + inv WF. ss. inv LOCAL. inv STEP. ss.
+      exploit PROMISES0; eauto. rewrite NOPROMISE, Promises.lookup_bot. ss.
+    + inv STEP. ss. esplits; ss.
+      funext. i. propext. econs; i.
+      * inv H; ss.
+      * left. ss.
+    + inv STEP. ss.
+    + inv STEP. ss.
+    + inv STEP. ss.
+    + inv STEP. ss.
+  - (* write step *)
+    admit.
+Admitted.
+
+Lemma no_promise_steps
+      tid aeu1 aeu2
+      (STEPS: rtc (AExecUnit.step tid) aeu1 aeu2)
+      (WF: ExecUnit.wf tid aeu1)
+      (NOPROMISE: aeu1.(ExecUnit.local).(Local.promises) = bot):
+  <<NOPROMISE: aeu2.(ExecUnit.local).(Local.promises) = bot>> /\
+  <<TAINT: aeu2.(AExecUnit.aux).(AExecUnit.taint) = aeu1.(AExecUnit.aux).(AExecUnit.taint)>>.
+Proof.
+  revert NOPROMISE. induction STEPS; ss. i.
+  exploit no_promise_step; eauto. i. des.
+  exploit IHSTEPS; eauto.
+  { admit. (* ExecUnit.wf after aeu step *) }
+  i. des.
+  esplits; ss. etrans; eauto.
+Admitted.
+
 Lemma rtc_state_step_certify_bot
       m1 m2 tid st lc
       (STEPS: rtc (Machine.step ExecUnit.state_step) m1 m2)
+      (WF: Machine.wf m1)
       (NOPROMISE: Machine.no_promise m2)
       (FIND: IdMap.find tid m1.(Machine.tpool) = Some (st, lc)):
   certify tid (ExecUnit.mk st lc m1.(Machine.mem)) bot.
@@ -35,6 +81,7 @@ Proof.
     - funext. unfold bot, fun_bot. i. propext. econs; ss. i. inv H; ss.
   }
   i. inv H. exploit IHSTEPS; ss.
+  { eapply Machine.step_state_step_wf; eauto. }
   { rewrite TPOOL, IdMap.add_spec, FIND.
     instantiate (1 := if equiv_dec tid tid0 then lc2 else lc).
     instantiate (1 := if equiv_dec tid tid0 then st2 else st).
